compiler/backend/passes/proofs/pure_letrec_spec_cexpProofScript.sml
@@ -1,0 +1,364 @@
+open HolKernel Parse boolLib bossLib;
+open fixedPointTheory arithmeticTheory listTheory stringTheory alistTheory
+     optionTheory pairTheory ltreeTheory llistTheory bagTheory dep_rewrite
+     BasicProvers pred_setTheory relationTheory rich_listTheory finite_mapTheory
+     combinTheory mlmapTheory indexedListsTheory;
+open pure_expTheory pure_valueTheory pure_evalTheory pure_eval_lemmasTheory
+     pure_exp_lemmasTheory pure_limitTheory pure_exp_relTheory
+     pure_miscTheory pure_letrec_delargTheory;
+open pure_cexpTheory pure_varsTheory balanced_mapTheory pureLangTheory;
+open pure_exp_relTheory pure_congruenceTheory
+open pure_inlineTheory pure_letrec_spec_cexpTheory
+
+val _ = new_theory "pure_letrec_spec_cexpProof";
+
+Theorem exp_of_SmartLam[simp]:
+  exp_of (SmartLam a vs x) = exp_of (Lam a vs x)
+Proof
+  rw [SmartLam_def] \\ Cases_on ‘vs’ \\ gvs [exp_of_def,Lams_def]
+QED
+
+Theorem exp_of_SmartApp[simp]:
+  exp_of (SmartApp a x xs) = exp_of (App a x xs)
+Proof
+  rw [SmartApp_def] \\ Cases_on ‘xs’ \\ gvs [exp_of_def,Apps_def]
+QED
+
+Theorem split_at_thm:
+  ∀n xs ys zs.
+    split_at n xs = (ys,zs) ∧ n ≤ LENGTH xs ⇒
+    xs = ys ++ zs ∧ LENGTH ys = n
+Proof
+  Induct \\ simp [Once split_at_def]
+  \\ Cases \\ fs [] \\ rw [] \\ pairarg_tac \\ gvs []
+  \\ res_tac \\ fs []
+QED
+
+Theorem drop_common_prefix_thm:
+  ∀xs ys xs1 ys1.
+    drop_common_prefix xs ys = (xs1,ys1) ⇒
+    ∃zs. xs = zs ++ xs1 ∧ ys = zs ++ ys1 ∧
+         (xs1 ≠ [] ∧ ys1 ≠ [] ⇒ HD xs1 ≠ HD ys1)
+Proof
+  Induct \\ Cases_on ‘ys’ \\ gvs [drop_common_prefix_def]
+  \\ rw [] \\ res_tac \\ fs []
+QED
+
+Theorem drop_common_suffix_thm:
+  ∀xs ys xs1 ys1.
+    drop_common_suffix xs ys = (xs1,ys1) ⇒
+    ∃zs. xs = xs1 ++ zs ∧ ys = ys1 ++ zs ∧
+         (xs1 ≠ [] ∧ ys1 ≠ [] ⇒ LAST xs1 ≠ LAST ys1)
+Proof
+  rw [drop_common_suffix_def]
+  \\ pairarg_tac \\ gvs []
+  \\ imp_res_tac drop_common_prefix_thm
+  \\ gvs [SWAP_REVERSE_SYM]
+  \\ gvs [GSYM SWAP_REVERSE_SYM,LAST_REVERSE]
+QED
+
+Theorem spec_one_thm:
+  (∀f v vs (e:'a cexp) e1 bs ts.
+     spec_one f v vs e = SOME e1 ∧
+     explode f ∉ boundvars (exp_of e) ∧
+     explode v ∉ boundvars (exp_of e) ∧
+     vs = MAP (K T) bs ++ [F] ++ MAP (K T) ts ⇒
+     can_spec_arg (explode f) bs (explode v) ts (exp_of e) (exp_of e1) ∧
+     boundvars (exp_of e1) ⊆ boundvars (exp_of e)) ∧
+  (∀f v vs (e:'a cexp list) e1 bs ts.
+     spec_one_list f v vs e = SOME e1 ∧
+     EVERY (λe. explode f ∉ boundvars (exp_of e)) e ∧
+     EVERY (λe. explode v ∉ boundvars (exp_of e)) e ∧
+     vs = MAP (K T) bs ++ [F] ++ MAP (K T) ts ⇒
+     LIST_REL (λe e1.
+       can_spec_arg (explode f) bs (explode v) ts (exp_of e) (exp_of e1) ∧
+       boundvars (exp_of e1) ⊆ boundvars (exp_of e)) e e1)
+Proof
+  cheat
+QED
+
+Triviality can_spec_arg_map:
+  ∀f vs v ws e1 e2.
+    can_spec_arg f vs v ws e1 e2 ⇒
+    can_spec_arg f (MAP explode vs) v (MAP explode ws) e1 e2
+Proof
+  ho_match_mp_tac can_spec_arg_ind \\ fs [] \\ rw []
+  \\ simp [Once can_spec_arg_cases] \\ gvs [SF ETA_ss]
+  \\ metis_tac []
+QED
+
+Triviality delete_with_lemma:
+  ∀xs ys.
+    delete_with (MAP (K T) xs ++ [F] ++ MAP (K T) ys) (xs ++ [h] ++ ys) = xs ++ ys
+Proof
+  Induct \\ fs [delete_with_def]
+  \\ Induct \\ fs [delete_with_def]
+QED
+
+Triviality MAP_NEQ:
+  ∀xs x. ¬MEM x xs ⇒ MAP (λv. x ≠ v) xs = MAP (K T) xs
+Proof
+  Induct \\ fs []
+QED
+
+Theorem specialise_each_thm:
+  ∀p args f c args1 c1.
+    specialise_each p args f c = (args1,c1) ∧
+    explode f ∉ boundvars (exp_of c) ∧
+    EVERY (λv. v ∉ boundvars (exp_of c)) (MAP explode args) ∧
+    ALL_DISTINCT p ∧ ALL_DISTINCT (MAP explode args) ∧
+    set p ⊆ set args ∧ ~MEM f args
+    ⇒
+    Letrec [(explode f,Lams (MAP explode args) (exp_of c))]
+      (Apps (Var (explode f)) (MAP Var (MAP explode args)))
+    ≅
+    Letrec [(explode f,Lams (MAP explode args1) (exp_of c1))]
+      (Apps (Var (explode f)) (MAP Var (MAP explode args1)))
+Proof
+  Induct \\ fs [specialise_each_def,exp_eq_refl]
+  \\ rpt gen_tac \\ IF_CASES_TAC \\ strip_tac \\ gvs [exp_eq_refl]
+  \\ gvs [CaseEq"bool"] \\ gvs [CaseEq"option"]
+  \\ ‘∃args1 args2. args = args1 ++ [h] ++ args2 ∧ ~MEM h args1 ∧ ~MEM h args2’ by
+   (qpat_x_assum ‘ALL_DISTINCT args’ mp_tac
+    \\ qpat_x_assum ‘MEM h args’ mp_tac
+    \\ qid_spec_tac ‘args’ \\ Induct
+    \\ fs [] \\ strip_tac \\ Cases_on ‘h = h'’ \\ gvs [] \\ rw []
+    >- (qexists_tac ‘[]’ \\ fs [])
+    \\ fs [] \\ qexists_tac ‘h'::args1'’ \\ fs [])
+  \\ gvs [MAP_NEQ]
+  \\ drule (CONJUNCT1 spec_one_thm |> SIMP_RULE std_ss [])
+  \\ impl_tac >- fs []
+  \\ strip_tac
+  \\ irule exp_eq_trans
+  \\ irule_at Any (letrec_spec_delarg |> SIMP_RULE std_ss [MAP_APPEND,MAP])
+  \\ irule_at Any can_spec_arg_map
+  \\ first_x_assum $ irule_at Any
+  \\ conj_tac >- (CCONTR_TAC \\ gvs [])
+  \\ conj_tac >- (gvs [ALL_DISTINCT_APPEND,MEM_MAP] \\ rw [] \\ gvs [])
+  \\ rewrite_tac [GSYM MAP_APPEND]
+  \\ last_x_assum irule \\ fs [delete_with_lemma]
+  \\ gvs [ALL_DISTINCT_APPEND,SUBSET_DEF,MEM_MAP,EVERY_MEM,PULL_EXISTS,SF SFY_ss]
+  \\ metis_tac []
+QED
+
+Triviality set_delete_with:
+  ∀args f. set (delete_with f args) ⊆ set args
+Proof
+  Induct \\ Cases_on ‘f’ \\ fs [delete_with_def]
+  \\ fs [SUBSET_DEF]
+  \\ Cases_on ‘h’ \\ fs [delete_with_def]
+  \\ rw [] \\ res_tac \\ fs []
+QED
+
+Theorem specialise_each_subset:
+  ∀p args f c args1 c1.
+    specialise_each p args f c = (args1,c1) ⇒
+    set args1 ⊆ set args
+Proof
+  Induct \\ fs [specialise_each_def] \\ rw []
+  \\ rw [] \\ res_tac \\ fs []
+  \\ gvs [AllCaseEqs()] \\ res_tac \\ fs []
+  \\ irule SUBSET_TRANS
+  \\ pop_assum $ irule_at Any
+  \\ fs [set_delete_with]
+QED
+
+Theorem no_shadowing_Lams_distinct:
+  ∀args x.
+    no_shadowing (Lams args x) ⇒
+    ALL_DISTINCT args
+Proof
+  Induct \\ simp [Once no_shadowing_cases,Lams_def]
+  \\ rw [] \\ res_tac \\ fs []
+  \\ pop_assum kall_tac \\ pop_assum mp_tac
+  \\ qid_spec_tac ‘args’ \\ Induct \\ fs [Lams_def]
+QED
+
+Theorem no_shadowing_Lams:
+  ∀args x.
+    no_shadowing (Lams args x) ⇒
+    EVERY (λv. v ∉ boundvars x) args
+Proof
+  Induct \\ simp [Once no_shadowing_cases,Lams_def]
+  \\ rw [] \\ pop_assum mp_tac
+  \\ qid_spec_tac ‘args’ \\ Induct \\ fs [Lams_def]
+QED
+
+Theorem LENGTH_const_call_args:
+  LENGTH (const_call_args f xs (c:'a cexp)) ≤ LENGTH xs
+Proof
+  qsuff_tac ‘
+      (∀f xs (c:'a cexp). LENGTH (const_call_args f xs c) ≤ LENGTH xs) ∧
+      (∀f xs (c:'a cexp list). LENGTH (const_call_args_list f xs c) ≤ LENGTH xs)’
+  >- fs []
+  \\ ho_match_mp_tac const_call_args_ind \\ rw []
+  \\ simp [Once const_call_args_def]
+  \\ rw [] \\ rpt (CASE_TAC \\ gvs [])
+  \\ irule LESS_EQ_TRANS
+  \\ pop_assum $ irule_at Any
+  \\ qid_spec_tac ‘c’
+  \\ qid_spec_tac ‘xs’
+  \\ ho_match_mp_tac min_call_args_ind
+  \\ fs [min_call_args_def] \\ rw []
+QED
+
+Theorem min_call_args_el:
+  ∀xs c i x.
+    EL i (min_call_args xs c) = SOME x ∧
+    i < LENGTH (min_call_args xs c)
+    ⇒
+    EL i xs = SOME x ∧ i < LENGTH xs
+Proof
+  ho_match_mp_tac min_call_args_ind
+  \\ rw [] \\ fs [min_call_args_def]
+  \\ Cases_on ‘i’ \\ fs [EL_MAP]
+  \\ FULL_CASE_TAC \\ gvs []
+QED
+
+Theorem const_call_args_el:
+  (∀f xs (c:'a cexp) i x.
+     i < LENGTH (const_call_args f xs c) ∧
+     EL i (const_call_args f xs c) = SOME x ⇒
+     EL i xs = SOME x ∧ i < LENGTH xs) ∧
+  (∀f xs (c:'a cexp list) i x.
+     i < LENGTH (const_call_args_list f xs c) ∧
+     EL i (const_call_args_list f xs c) = SOME x ⇒
+     EL i xs = SOME x ∧ i < LENGTH xs)
+Proof
+  ho_match_mp_tac const_call_args_ind
+  \\ reverse $ rpt conj_tac
+  \\ rpt gen_tac
+  \\ rpt disch_tac
+  \\ fs [const_call_args_def] \\ fs []
+  \\ fs [SF SFY_ss]
+  \\ rw [] \\ rpt (CASE_TAC \\ gvs [])
+  \\ rw [] \\ rpt (FULL_CASE_TAC \\ gvs [])
+  \\ res_tac \\ fs []
+  \\ fs [const_call_args_def] \\ fs []
+  >- metis_tac []
+  \\ drule_all min_call_args_el \\ fs []
+QED
+
+Triviality MEM_all_somes:
+  ∀xs x. MEM x (all_somes xs) = MEM (SOME x) xs
+Proof
+  Induct \\ fs [all_somes_def]
+  \\ Cases \\ fs [all_somes_def]
+QED
+
+Theorem MEM_min_call_args:
+  ∀xs c x.
+    MEM x (all_somes (min_call_args xs c)) ⇒
+    MEM x (all_somes xs)
+Proof
+  ho_match_mp_tac min_call_args_ind \\ rw []
+  \\ fs [min_call_args_def,all_somes_def]
+  \\ rpt (FULL_CASE_TAC \\ gvs [])
+  \\ gvs [all_somes_def] \\ fs [MEM_all_somes,MEM_MAP]
+QED
+
+Theorem const_call_args_distinct:
+  (∀f xs (c:'a cexp).
+     ALL_DISTINCT (all_somes xs) ⇒
+     ALL_DISTINCT (all_somes (const_call_args f xs c))) ∧
+  (∀f xs (c:'a cexp list).
+     ALL_DISTINCT (all_somes xs) ⇒
+     ALL_DISTINCT (all_somes (const_call_args_list f xs c)))
+Proof
+  ho_match_mp_tac const_call_args_ind \\ rw []
+  \\ fs [const_call_args_def] \\ fs []
+  \\ rw [] \\ rpt (FULL_CASE_TAC \\ gvs [])
+  \\ fs [const_call_args_def] \\ fs [all_somes_def]
+  \\ pop_assum irule
+  \\ pop_assum mp_tac
+  \\ qid_spec_tac ‘c’
+  \\ qid_spec_tac ‘xs’
+  \\ ho_match_mp_tac min_call_args_ind
+  \\ fs [min_call_args_def,all_somes_def] \\ rw []
+  \\ fs [min_call_args_def,all_somes_def] \\ rw []
+  \\ CCONTR_TAC \\ fs []
+  \\ imp_res_tac MEM_min_call_args
+QED
+
+Triviality all_somes_map_some:
+  ∀xs. all_somes (MAP SOME xs) = xs
+Proof
+  Induct \\ fs [all_somes_def]
+QED
+
+Theorem specialise_thm:
+  specialise f e = SOME out ∧
+  no_shadowing (exp_of (Lam a [f] e)) ∧
+  NestedCase_free e
+  ⇒
+  exp_of (Letrec a [(f,e)] rest)
+  ≅
+  exp_of (Let a f out rest)
+Proof
+  fs [exp_of_def,Lams_def]
+  \\ Cases_on ‘e’ \\ fs [specialise_def]
+  \\ strip_tac \\ gvs [exp_of_def,boundvars_Lams,MEM_MAP]
+  \\ rpt (pairarg_tac \\ gvs [])
+  \\ drule split_at_thm
+  \\ impl_tac >-
+   (irule LESS_EQ_TRANS
+    \\ irule_at Any LENGTH_const_call_args \\ fs [])
+  \\ strip_tac
+  \\ gvs [Lams_append]
+  \\ qabbrev_tac ‘c1 = SmartLam a ws2 c’
+  \\ qabbrev_tac ‘guide = const_call_args f (MAP SOME ws1 ++ MAP SOME ws2) c’
+  \\ ‘Lams (MAP explode ws2) (exp_of c) = exp_of c1’ by fs [exp_of_def,Abbr‘c1’]
+  \\ fs []
+  \\ irule exp_eq_trans
+  \\ irule_at (Pos hd) Letrec_expand_1 \\ fs [MEM_MAP]
+  \\ irule exp_eq_App_cong \\ fs [exp_eq_refl]
+  \\ fs [MAP_MAP_o,combinTheory.o_DEF,exp_of_def]
+  \\ gvs [MEM_MAP,exp_of_def]
+  \\ drule drop_common_suffix_thm
+  \\ strip_tac
+  \\ pop_assum kall_tac
+  \\ gvs [MAP_MAP_o,combinTheory.o_DEF,exp_of_def]
+  \\ ‘∀xs. MAP (λx. pure_exp$Var (explode x)) xs = MAP Var (MAP explode xs)’ by
+       fs [MAP_MAP_o,combinTheory.o_DEF,exp_of_def] \\ fs []
+  \\ irule exp_eq_trans
+  \\ irule_at (Pos last) Letrec_contract_1
+  \\ gvs [MEM_MAP]
+  \\ rewrite_tac [GSYM MAP_APPEND]
+  \\ conj_tac >-
+   (imp_res_tac specialise_each_subset
+    \\ fs [SUBSET_DEF] \\ CCONTR_TAC \\ gvs [] \\ res_tac)
+  \\ irule Lams_cong
+  \\ full_simp_tac bool_ss [GSYM MAP_APPEND]
+  \\ imp_res_tac no_shadowing_Lams
+  \\ imp_res_tac no_shadowing_Lams_distinct
+  \\ irule specialise_each_thm \\ simp []
+  \\ first_x_assum $ irule_at Any \\ fs []
+  \\ conj_tac >- (fs [Abbr‘c1’,exp_of_def,boundvars_Lams,MEM_MAP])
+  \\ simp [SUBSET_DEF,MEM_all_somes]
+  \\ conj_tac
+  >-
+   (unabbrev_all_tac
+    \\ irule (const_call_args_distinct |> CONJUNCT1)
+    \\ rewrite_tac [GSYM MAP_APPEND,all_somes_map_some]
+    \\ ‘no_shadowing (exp_of (Lam a (outer_vs ++ zs ++ ws2) c))’ by
+         fs [exp_of_def,Lams_append]
+    \\ fs [exp_of_def]
+    \\ drule no_shadowing_Lams_distinct
+    \\ rewrite_tac [GSYM MAP_APPEND]
+    \\ metis_tac [ALL_DISTINCT_MAP])
+  \\ qsuff_tac ‘∀x. MEM (SOME x) guide ⇒ MEM x (outer_vs ++ zs)’ >- fs []
+  \\ qabbrev_tac ‘zs1 = outer_vs ++ zs’
+  \\ simp [MEM_EL] \\ strip_tac \\ strip_tac
+  \\ pop_assum $ assume_tac o GSYM
+  \\ unabbrev_all_tac
+  \\ drule_all (const_call_args_el |> CONJUNCT1)
+  \\ gvs [] \\ strip_tac
+  \\ qexists_tac ‘n’ \\ fs []
+  \\ ‘n < LENGTH (outer_vs ++ zs)’ by fs []
+  \\ qpat_x_assum ‘_ = SOME x’ mp_tac
+  \\ rewrite_tac [GSYM MAP_APPEND] \\ simp [EL_MAP]
+  \\ strip_tac \\ rw []
+  \\ metis_tac [EL_APPEND1]
+QED
+
+val _ = export_theory();
